EC Signed DH: step 0, pen-and-paper style

signedDH/easycrypt/SignedDH.ec
@@ -27,9 +27,6 @@ require (*--*) St_CDH_abstract SUFCMA UATPaKE.
      RO.
 *)
 
-(** Handles to refer to servers and client instances **)
-type s_handle, c_handle.
-
 (** Types and operators for the DH group **)
 type pdh, sdh, sskey.
 
@@ -136,3 +133,228 @@ module SignedDH (S : SigScheme) (H : RO) : UATPaKE = {
     return r;
   }
 }.
+
+section.
+declare module S <: SigScheme { -Exp_b, -RO }.
+declare module A <: Adv_UATPaKE_RO { -Exp_b, -RO, -S }.
+
+local module Game0_b = {
+  (* The challenge bit *)
+  var b_ror : bool
+
+  (* Server maps: *)
+  var m: int
+  (* - server handle to keypair *)
+  var pk_map: (int, pkey) fmap
+  var sk_map: (int, skey) fmap
+  (* - server-client handle to partial trace *)
+  var r_map: (int option * int, (pdh * sig) fset) fmap
+
+  (* Client maps: *)
+  var n: int
+  (* - client handle to state *)
+  var c_map: (int, client_state) fmap
+  (* - client handle to intended partner *)
+  var p_map: (int, int) fmap
+  (* - client handle to partial trace (early partnering) *)
+  var i_map: (int, pdh) fmap
+
+  var q   : int fset
+  var ich : int fset
+  var rch : int fset
+  var xp  : int fset
+  var cr  : int fset
+
+  module Oracles = {
+    proc gen(): pkey = {
+      var pk, sk;
+
+      m <- m + 1;
+      (pk, sk) <@ S.keygen();
+      pk_map.[m] <- pk;
+      sk_map.[m] <- sk;
+      return pk;
+    }
+
+    proc corrupt(j: int): skey option = {
+      var r <- None;
+
+      if (0 < j <= m) {
+        r <- sk_map.[j];
+        cr <- cr `|` fset1 j;
+      }
+      return r;
+    }
+
+    proc expose(i) = {
+      var r <- None;
+
+      if (0 < i <= n /\ i \notin ich) {
+        xp <- xp `|` fset1 i;
+        r <- c_map.[i];
+      }
+      return r;
+    }
+
+    proc init(pk: pkey): pdh = {
+      var st, jo, c, x;
+
+      n <- n + 1;
+      (c, x) <$ dkp;
+      st <- {| s_id = pk; x_pk = c; x_sk = x |};
+      c_map.[n] <- st;
+      jo <- find (fun _ pk_j=> pk_j = pk) pk_map;
+      if (jo is Some j) {
+        p_map.[n] <- j;
+        i_map.[n] <- c;
+      }
+      return c;
+    }
+
+    proc respond(j: int, c: pdh, ch: bool): (sskey * (pdh * sig)) option = {
+      var k, c', io, sk_j, h, y, sig;
+      var r <- None;
+
+      if (0 < j <= m) {
+        sk_j <- oget sk_map.[j];
+        (h, y) <$ dkp;
+        sig <@ S.sign(sk_j, (c, h));
+        c' <- (h, sig);
+        k <@ RO.get(shared_key c y, c, h);
+        io <- find (fun i _=> p_map.[i] = Some j /\ i_map.[i] = Some c) c_map;
+        if (io is Some i) {
+          (*** Instead of initialising all of r_map to output the
+          empty set, we read undefined entries as the empty set
+          here. ***)
+          r_map.[Some j, i] <- (odflt fset0 r_map.[Some j, i]) `|` fset1 c';
+          if (ch /\ i \notin xp) {
+            if (b_ror) { k <$ dssk; }
+            ich <- ich `|` fset1 i;
+          }
+        }
+        r <- Some (k, c');
+      }
+      return r;
+    }
+
+    proc receive(i: int, c: pdh * sig, ch: bool): sskey option = {
+      var st_i, k, h, sig, b;
+      var ko <- None;
+
+      if (0 < i <= n /\ i \notin q) {
+        st_i <- oget c_map.[i];
+        q <- q `|` fset1 i;
+        
+        if (c \notin odflt fset0 r_map.[p_map.[i], i]) {
+          (h, sig) <- c;
+          b <@ S.verify(s_id st_i, (x_pk st_i, h), sig);
+          if (b) {
+            k <@ RO.get(shared_key h (x_sk st_i), x_pk st_i, h);
+            ko <- Some k;
+          }
+          if (   ch
+              /\ i \notin xp
+              /\ p_map.[i] <> None /\ 0 < oget p_map.[i] <= m /\ oget p_map.[i] \notin cr
+              /\ ko <> None) {
+            if (b_ror) { k <$ dssk; ko <- Some k; }
+            ich <- ich `|` fset1 i;
+          }
+        }
+      }
+      return ko;
+    }
+
+    proc h = RO.get
+  }
+
+  proc run(b) = {
+    var b';
+
+    RO.init();
+
+    b_ror <- b;
+
+    m <- 0;
+    n <- 0;
+
+    q <- fset0;
+    ich <- fset0;
+    rch <- fset0;
+    xp <- fset0;
+    cr <- fset0;
+
+    p_map <- empty;
+    i_map <- empty;
+    r_map <- empty;
+
+    pk_map <- empty;
+    sk_map <- empty;
+    c_map <- empty;
+
+    b' <@ A(Oracles).distinguish();
+    return b';
+  }
+}.
+
+local lemma Hop0 &m:
+  `|  Pr[Exp_b(SignedDH(S), RO, A).run(false) @ &m: res]
+    - Pr[Exp_b(SignedDH(S), RO, A).run(true ) @ &m: res] |
+  = `|  Pr[Game0_b.run(false) @ &m: res]
+      - Pr[Game0_b.run(true ) @ &m: res] |.
+proof.
+have ^ + -> - -> //:
+  forall b, Pr[Exp_b(SignedDH(S), RO, A).run(b) @ &m: res]
+          = Pr[Game0_b.run(b) @ &m: res].
+move=> b; byequiv (: ={glob A, glob S, arg} ==> ={res})=> //.
+proc.
+(* The calls are equivalent due to equality on a bunch of variables *)
+call (: ={glob S, glob RO, b_ror, m, n, q, ich, rch, xp, cr,
+          c_map, p_map, i_map, r_map, pk_map, sk_map}(Exp_b, Game0_b));
+  last first.
+(* The invariant holds initially and allows us to conclude *)
++ by inline *; auto.
+(* The invariant is preserved by all oracles *)
++ by proc; inline *; auto; call (: true); auto.
++ by proc; inline *; auto.
++ by proc; inline *; auto.
++ proc; inline *.
+  swap {1} 3 -2. swap {2} 2 -1.
+  seq 1 1: (#pre /\ (x_pk, x_sk){1} = (c, x){2}).
+  + by auto.
+  sp 5 4. match =; 1,2:by auto.
+  by move=> j; auto.
++ proc; inline *; sp; if; auto.
+  swap {1} 4 -3. swap {2} 2 -1.
+  swap {1} 8 -7. swap {2} 6 -5.
+  seq 2 2: (#pre /\ (y_pk, y_sk){1} = (h, y){2} /\ ={r0}).
+  + by auto.
+  sp; seq 1 1: (#pre /\ s{1} = sig{2}).
+  + by call (: true).
+  sp 2 2.
+  seq 1 1: #pre.
+  + by auto.
+  sp 3 2.
+  match =; 1,2:by auto.
+  by move=> i; sp; if; auto; if; auto.
++ proc; sp; if; auto; sp; if; auto.
+  inline {1} 1.
+  sp; seq 1 1: (#pre /\ ={b}).
+  + call (: true); auto=> /> &2.
+    move=> qR _ _ i_notin_qR _; exists qR=> //=.
+    by exists qR.
+  if; 1:by auto.
+  + sp; seq 1 1: (#pre /\ kc{1} = k{2}).
+    + call (: ={glob RO, arg} ==> ={glob RO, res}).
+      + by sim.
+      auto=> /> &2 qR _ _ i_notin_qR _ _; exists qR=> //=.
+      by exists qR.
+    sp; if; auto.
+    by if; auto.
+  rcondf {1} 2; 1:by auto.
+  rcondf {2} 1; 1:by auto.
+  by auto.
++ conseq (: _ ==> ={glob RO, res})=> //.
+  by sim.
+qed.
+
+end section.
